code/hash/Lib.IntTuple.fst
@@ -6,53 +6,53 @@ open Lib.NTuple
 
 #set-options "--z3rlimit 100"
 let funit (i:nat) = unit
-let ntuple_to_bytes_be (#t:inttype{unsigned t}) (#l:secrecy_level) (#len:flen) (s:ntuple (uint_t t l) len) : Lib.ByteSequence.lbytes_l l (numbytes t * len) =
+let ntuple_to_bytes_be (#t:inttype{unsigned t}) (#l:secrecy_level) (#len:flen{numbytes t * len <= max_size_t}) (s:ntuple (uint_t t l) len) : Lib.ByteSequence.lbytes_l l (numbytes t * len) =
     assert_norm (len * numbytes t < pow2 32);
     let _, o = normalize_term (Lib.Sequence.generate_blocks (numbytes t) len len funit
 		(fun i u -> (),Lib.ByteSequence.uint_to_bytes_be #t #l s.(|i|)) ()) in
     o
 
-let ntuple_to_bytes_le (#t:inttype{unsigned t}) (#l:secrecy_level) (#len:flen) (s:ntuple (uint_t t l) len) : Lib.ByteSequence.lbytes_l l (numbytes t * len) =
+let ntuple_to_bytes_le (#t:inttype{unsigned t}) (#l:secrecy_level) (#len:flen{numbytes t * len <= max_size_t}) (s:ntuple (uint_t t l) len) : Lib.ByteSequence.lbytes_l l (numbytes t * len) =
     assert_norm (len * numbytes t < pow2 32);
     let _, o = normalize_term (Lib.Sequence.generate_blocks (numbytes t) len len funit
 		(fun i u -> (),Lib.ByteSequence.uint_to_bytes_le #t #l s.(|i|)) ()) in
     o
 
-let ntuple_from_bytes_be (#t:inttype{unsigned t /\ t <> U1}) (#l:secrecy_level) (#len:flen) (b:Lib.ByteSequence.lbytes_l l (numbytes t * len)) : (s:ntuple (uint_t t l) len) =
+let ntuple_from_bytes_be (#t:inttype{unsigned t /\ t <> U1}) (#l:secrecy_level) (#len:flen{numbytes t * len <= max_size_t}) (b:Lib.ByteSequence.lbytes_l l (numbytes t * len)) : (s:ntuple (uint_t t l) len) =
     normalize_term (createi #(uint_t t l) len
       (fun i -> Lib.ByteSequence.uint_from_bytes_be (Lib.Sequence.sub b (i * numbytes t) (numbytes t))))
 
-let ntuple_from_bytes_le (#t:inttype{unsigned t /\ t <> U1}) (#l:secrecy_level) (#len:flen) (b:Lib.ByteSequence.lbytes_l l (numbytes t * len)) : (s:ntuple (uint_t t l) len) =
+let ntuple_from_bytes_le (#t:inttype{unsigned t /\ t <> U1}) (#l:secrecy_level) (#len:flen{numbytes t * len <= max_size_t}) (b:Lib.ByteSequence.lbytes_l l (numbytes t * len)) : (s:ntuple (uint_t t l) len) =
     normalize_term (createi #(uint_t t l) len
       (fun i -> Lib.ByteSequence.uint_from_bytes_le (Lib.Sequence.sub b (i * numbytes t) (numbytes t))))
 
 inline_for_extraction
-let (+|) #t #l #len = map2 #(uint_t t l) #(uint_t t l) #(uint_t t l) #len ( +. )
+let (+*) #t #l #len = map2 #(uint_t t l) #(uint_t t l) #(uint_t t l) #len ( +. )
 
 inline_for_extraction
-let ( *| ) (#t:inttype{unsigned t /\ t <> U128}) #l #len = map2 #(uint_t t l) #(uint_t t l) #(uint_t t l) #len ( *. )
+let ( ** ) (#t:inttype{unsigned t /\ t <> U128}) #l #len = map2 #(uint_t t l) #(uint_t t l) #(uint_t t l) #len ( *. )
 
 inline_for_extraction
-let (-|) #t #l #len = map2 #(uint_t t l) #(uint_t t l) #(uint_t t l) #len ( -. )
+let (-*) #t #l #len = map2 #(uint_t t l) #(uint_t t l) #(uint_t t l) #len ( -. )
 
 inline_for_extraction
-let (^|) #t #l #len = map2 #(uint_t t l) #(uint_t t l) #(uint_t t l) #len ( ^. )
+let (^*) #t #l #len = map2 #(uint_t t l) #(uint_t t l) #(uint_t t l) #len ( ^. )
 
 inline_for_extraction
-let (&|) #t #l #len = map2 #(uint_t t l) #(uint_t t l) #(uint_t t l) #len ( &. )
+let (&*) #t #l #len = map2 #(uint_t t l) #(uint_t t l) #(uint_t t l) #len ( &. )
 
 inline_for_extraction
-let (~|) #t #l #len = map #(uint_t t l) #(uint_t t l) #len ( ~. )
+let (~*) #t #l #len = map #(uint_t t l) #(uint_t t l) #len ( ~. )
 
 inline_for_extraction
-let (>>>|) #t #l #len x r  = map #(uint_t t l) #(uint_t t l) #len ( fun i -> i >>>. r ) x
+let (>>>*) #t #l #len x r  = map #(uint_t t l) #(uint_t t l) #len ( fun i -> i >>>. r ) x
 
 inline_for_extraction
-let (>>|) #t #l #len x r  = map #(uint_t t l) #(uint_t t l) #len ( fun i -> i >>. r ) x
+let (>>*) #t #l #len x r  = map #(uint_t t l) #(uint_t t l) #len ( fun i -> i >>. r ) x
 
 inline_for_extraction
-let (<<<|) #t #l #len x r  = map #(uint_t t l) #(uint_t t l) #len ( fun i -> i <<<. r ) x
+let (<<<*) #t #l #len x r  = map #(uint_t t l) #(uint_t t l) #len ( fun i -> i <<<. r ) x
 
 inline_for_extraction
-let (<<|) #t #l #len x r  = map #(uint_t t l) #(uint_t t l) #len ( fun i -> i <<. r ) x
+let (<<*) #t #l #len x r  = map #(uint_t t l) #(uint_t t l) #len ( fun i -> i <<. r ) x
 
